finished the HNR_while rule

Example.thy
@@ -2,8 +2,22 @@ theory Example
 imports HNR  
 begin
 
+subsection "Mono Prover"
+
+  (* Wraps mono-prover of partial-function to erase premises. 
+    This is a workaround for mono_tac, which does not accept premises if the case-split rule is applied. *)
 
 
+ML \<open>
+  structure Pf_Mono_Prover = struct
+    fun mono_tac ctxt = (REPEAT o eresolve_tac ctxt @{thms thin_rl})
+      THEN' Partial_Function.mono_tac ctxt
+  end
+\<close>
+
+method_setup pf_mono = \<open>Scan.succeed (fn ctxt => SIMPLE_METHOD' (Pf_Mono_Prover.mono_tac ctxt))\<close> \<open>Monotonicity prover of the partial function package\<close>
+
+subsection "While rule for hnr"
 
 definition "monadic_WHILEIT I b f s \<equiv> do {
   Sepreftime.RECT (\<lambda>D s. do {
@@ -22,7 +36,7 @@ definition "heap_WHILET b f s \<equiv> do {
     if bv then do {
       s \<leftarrow> f s;
       D s
-    } else do {return s}
+    } else do {ureturn s}
   }) s
 }"
 
@@ -33,25 +47,152 @@ lemma heap_WHILET_unfold[code]: "heap_WHILET b f s =
       s \<leftarrow> f s;
       heap_WHILET b f s
     } else
-      return s
+      ureturn s
   }"
   unfolding heap_WHILET_def
   apply (subst heap.mono_body_fixp)
-  subgoal sorry
+  apply pf_mono
   apply simp
   done
 
-definition "WHILEIT I b c s = whileT b c s"
 
+definition  WHILEIT :: "('a \<Rightarrow> bool) \<Rightarrow> ('a \<Rightarrow> bool) \<Rightarrow> ('a \<Rightarrow> 'a nrest) \<Rightarrow> 'a \<Rightarrow> 'a nrest" where
+  " WHILEIT I b c = RECT (\<lambda>whileT s. (if I s then (if b s then bindT (c s) whileT else RETURNT s) else FAILT))"
+ 
 lemma WHILEIT_to_monadic: "WHILEIT I b f s = monadic_WHILEIT I (\<lambda>s. RETURNT (b s)) f s"
   unfolding WHILEIT_def monadic_WHILEIT_def
   unfolding whileT_def bind_ASSERT_eq_if
-  apply (simp cong: if_cong) sorry
+  by (simp cong: if_cong) 
 
 lemma Ra: "A * \<Gamma> \<Longrightarrow>\<^sub>t \<Gamma> * A"  
   by (simp add: assn_times_comm entt_refl)  
 
 
+
+lemma left_move_back: "(A \<Longrightarrow>\<^sub>A B * C) \<Longrightarrow> (A \<Longrightarrow>\<^sub>A C * B)"
+  by (simp add: assn_times_comm)
+lemma right_move_back: "(B * C \<Longrightarrow>\<^sub>A A) \<Longrightarrow> (C * B \<Longrightarrow>\<^sub>A A)"
+  by (simp add: assn_times_comm)
+
+lemma pull_forward: "(A \<Longrightarrow>\<^sub>A B * C * D) \<Longrightarrow> (A \<Longrightarrow>\<^sub>A B * (C * D))"
+  by (simp add: mult.assoc)
+
+lemma match_first: "A \<Longrightarrow>\<^sub>A B \<Longrightarrow> \<Gamma> * A \<Longrightarrow>\<^sub>A \<Gamma> * B"  
+  by (simp add: assn_times_comm entails_frame)  
+
+lemma match_rest: "emp \<Longrightarrow>\<^sub>A B \<Longrightarrow> \<Gamma> \<Longrightarrow>\<^sub>A \<Gamma> * B"  
+  using match_first by fastforce 
+
+thm mult.assoc
+method rotater = ( (simp add: mult.assoc)? , rule left_move_back , (simp add: mult.assoc)?  )
+method rotatel = ( (simp add: mult.assoc)? , rule right_move_back , (simp add: mult.assoc)?  )
+
+lemma "\<And>x y. A \<Longrightarrow>\<^sub>A B x y * C"
+  apply rotater
+  oops
+ 
+schematic_goal "\<And>x y. A \<Longrightarrow>\<^sub>A B x y * ?C x " 
+  apply rotater
+  oops
+
+lemma "A \<Longrightarrow>\<^sub>A B * D * E * F"  
+  apply rotater
+  oops
+
+ 
+
+
+lemma assumes "hn_refine P c Q R a"
+    "Q\<Longrightarrow>\<^sub>AQ'*true" shows "hn_refine P c Q' R a"
+  apply(rule hn_refine_cons'[OF _ assms]) by (auto simp add: entt_refl') 
+
+
+text \<open>Weakening the postcondition by converting @{const invalid_assn} to @{term "\<lambda>_ _. true"}\<close>
+definition "WEAKEN_HNR_POST \<Gamma> \<Gamma>' \<Gamma>'' \<equiv> (\<exists>h. h\<Turnstile>\<Gamma>) \<longrightarrow> (\<Gamma>'' \<Longrightarrow>\<^sub>t \<Gamma>')"
+
+lemma weaken_hnr_postI:
+  assumes "WEAKEN_HNR_POST \<Gamma> \<Gamma>'' \<Gamma>'"
+  assumes "hn_refine \<Gamma> c \<Gamma>' R a"
+  shows "hn_refine \<Gamma> c \<Gamma>'' R a"
+  apply (rule hn_refine_preI)
+  apply (rule hn_refine_cons_post)
+  apply (rule assms)
+  using assms(1) unfolding WEAKEN_HNR_POST_def by blast
+
+lemma weaken_hnr_post_triv: "WEAKEN_HNR_POST \<Gamma> P P"
+  unfolding WEAKEN_HNR_POST_def  
+  using entt_refl by blast  
+
+lemma weaken_hnr_post:
+  "\<lbrakk>WEAKEN_HNR_POST \<Gamma> P P'; WEAKEN_HNR_POST \<Gamma>' Q Q'\<rbrakk> \<Longrightarrow> WEAKEN_HNR_POST (\<Gamma>*\<Gamma>') (P*Q) (P'*Q')"
+  "WEAKEN_HNR_POST (hn_ctxt R x y) (hn_ctxt R x y) (hn_ctxt R x y)"
+  "WEAKEN_HNR_POST (hn_ctxt R x y) (hn_invalid R x y) (hn_ctxt (\<lambda>_ _. true) x y)"
+proof (goal_cases)
+  case 1 thus ?case
+    unfolding WEAKEN_HNR_POST_def
+    apply clarsimp  
+  proof -
+    fix h :: pheap
+    assume a1: "h \<Turnstile> \<Gamma> * \<Gamma>'"
+    assume a2: "(\<exists>h. h \<Turnstile> \<Gamma>) \<longrightarrow> (P' \<Longrightarrow>\<^sub>t P)"
+    assume a3: "(\<exists>h. h \<Turnstile> \<Gamma>') \<longrightarrow> (Q' \<Longrightarrow>\<^sub>t Q)"
+have f4: "\<forall>a. h \<Turnstile> a * (\<Gamma>' * \<up> (h \<Turnstile> \<Gamma> * \<Gamma>')) \<or> (P' \<Longrightarrow>\<^sub>t P)"
+  using a2 a1 by (metis (no_types) SepAuto.mod_pure_star_dist assn_times_assoc entailsD' entailsI)
+  have f5: "\<forall>b a aa p. p \<Turnstile> aa * a \<or> \<not> p \<Turnstile> aa * (a * \<up> b)"
+by (metis (no_types) SepAuto.mod_pure_star_dist assn_times_assoc)
+then have f6: "\<forall>b. (P' \<Longrightarrow>\<^sub>t P) \<or> b"
+  using f4 by (metis SepAuto.mod_pure_star_dist mult.left_commute)
+  then have "h \<Turnstile> \<Gamma> * (\<Gamma>' * \<up> (P' \<Longrightarrow>\<^sub>t P))"
+    using a1 by (metis (full_types) SepAuto.mod_pure_star_dist assn_times_assoc)
+  then have f7: "Q' \<Longrightarrow>\<^sub>A Q * true"
+    using f5 a3 by (metis SepAuto.mod_pure_star_dist entailsD' entailsI entailst_def mult.left_commute)
+  have "\<forall>a. true * (a * true) = a * true"
+    by (simp add: mult.left_commute)
+  then have "P' * Q' \<Longrightarrow>\<^sub>A P * (Q * true)"
+using f7 f6 by (metis (no_types) assn_times_assoc ent_star_mono entailst_def)
+then show "P' * Q' \<Longrightarrow>\<^sub>t P * Q"
+  by (simp add: assn_times_assoc entailst_def)
+qed  (* thank you sledgehammer :) *)
+next
+  case 2 thus ?case by (rule weaken_hnr_post_triv)
+next
+  case 3 thus ?case 
+    unfolding WEAKEN_HNR_POST_def  invalid_assn_def hn_ctxt_def
+     
+    using assn_times_comm ent_imp_entt entails_pure_post by fastforce   
+qed
+
+
+ML \<open>
+
+  fun weaken_post_tac ctxt = TRADE (fn ctxt =>
+    resolve_tac ctxt @{thms weaken_hnr_postI} 
+    THEN' SOLVED' (REPEAT_ALL_NEW (DETERM o resolve_tac ctxt @{thms weaken_hnr_post weaken_hnr_post_triv}))
+  ) ctxt
+
+\<close>
+
+
+method_setup weaken_hnr_post = \<open>Scan.succeed (fn ctxt => SIMPLE_METHOD'  (weaken_post_tac ctxt))\<close>
+  \<open>Convert "hn_invalid" to "hn_ctxt (\<lambda>_ _. true)" in postcondition of hn_refine goal\<close>
+
+
+lemma ent_disjE: "\<lbrakk> A\<Longrightarrow>\<^sub>AC; B\<Longrightarrow>\<^sub>AC \<rbrakk> \<Longrightarrow> A\<or>\<^sub>AB \<Longrightarrow>\<^sub>AC"
+  unfolding entails_def sorry
+
+
+lemma merge_true_star_ctx: "true * (true * P) = true * P"
+  by (metis assn_times_assoc top_assn_reduce)
+
+lemma pf: "(a::assn) * b = b * a" 
+  using assn_times_comm by auto 
+
+lemma ent_true_drop: 
+  "P\<Longrightarrow>\<^sub>AQ*true \<Longrightarrow> P*R\<Longrightarrow>\<^sub>AQ*true"
+  "P\<Longrightarrow>\<^sub>AQ \<Longrightarrow> P\<Longrightarrow>\<^sub>AQ*true"
+  apply (metis assn_times_comm ent_star_mono ent_true merge_true_star_ctx)
+  apply (metis assn_one_left ent_star_mono ent_true pf)
+  done
 
 lemma hn_monadic_WHILE_aux:
   assumes FR: "P \<Longrightarrow>\<^sub>t \<Gamma> * hn_ctxt Rs s' s"
@@ -72,9 +213,12 @@ lemma hn_monadic_WHILE_aux:
   assumes f_fr: "\<And>s' s. \<Gamma>f s' s \<Longrightarrow>\<^sub>t \<Gamma> * hn_ctxt (\<lambda>_ _. true) s' s"
   (*assumes PREC: "precise Rs"*)
   shows "hn_refine (P) (heap_WHILET b f s) (\<Gamma> * hn_invalid Rs s' s) Rs (monadic_WHILEIT I b' f' s')"
-
+  
   unfolding monadic_WHILEIT_def heap_WHILET_def
   apply1 (rule hn_refine_cons_pre[OF FR]) 
+  
+  apply weaken_hnr_post
+
   focus (rule hn_refine_cons_pre[OF _ hnr_RECT])
     applyS (subst mult_ac(2)[of \<Gamma>]; rule entt_refl; fail)
 
@@ -96,40 +240,46 @@ lemma hn_monadic_WHILE_aux:
       
           focus (rule hn_refine_frame)
             applyS rprems
-            apply  (rule enttI; solve_entails)
+            apply  (rule enttI)
+            apply(simp add: mult_ac ) 
+              apply rotater 
+              apply(rule match_first)
+              apply(rule match_first)
+              apply(rule match_rest) apply simp 
           solved
-  
-          apply (sep_auto intro!: enttI; fail)
-        solved  
-        applyF (sep_auto,rule hn_refine_frame)
-          applyS (rule hnr_RETURN_pass)
+          
+          apply rotatel apply rotatel apply rotater
+              apply(rule match_first)  apply rotater
+              apply(rule match_rest) apply simp
+            solved   
+        applyF (auto,rule hn_refine_frame)
+          applyS (rule hnr_uRETURN_pass)
           (*apply (tactic {* Sepref_Frame.frame_tac @{context} 1*})*)
           apply (rule enttI)
-          apply (fr_rot_rhs 1)
-          apply (fr_rot 1, rule fr_refl)
-          apply (rule fr_refl)
-          apply solve_entails
+          apply rotatel  apply rotater  
+              apply(rule match_first) apply rotater 
+              apply(rule match_rest) apply simp
         solved
 
         apply (rule entt_refl)
       solved  
 
-      apply (rule enttI)
-      applyF (rule ent_disjE)
-        apply1 (sep_auto simp: hn_ctxt_def pure_def)
-        apply1 (rule ent_true_drop)
-        apply1 (rule ent_true_drop)
-        applyS (rule ent_refl)
-        
-        applyS (sep_auto simp: hn_ctxt_def pure_def)
+            applyF (rule ent_disjE) apply(simp only: hn_ctxt_def)
+             apply rotatel apply (rule match_first) apply rotater 
+             apply (rule match_rest) apply simp 
+
+            apply(simp only: hn_ctxt_def)
+
+        apply1 (rule ent_true_drop) apply rotatel 
+        apply1 (rule match_first) 
+             
+            apply simp
+         
       solved    
     solved
     apply pf_mono
   solved
-  done 
-  sorry
-  sorry
-  oops
+  done  
 
 (* monotonicity *)
 thm bindT_mono
@@ -144,6 +294,10 @@ lemma k: "(emp \<Longrightarrow>\<^sub>A \<up> (s = S) * true) \<longleftrightar
   apply rule
   apply (smt assn_ext entailsD' entailsI mod_false' mult.left_neutral pure_assn_eq_conv)   
   using assn_times_comm entails_pure_post entails_true by fastforce
+lemma k2: "(emp \<Longrightarrow>\<^sub>A \<up> (s = S) ) \<longleftrightarrow> s=S" 
+  apply rule
+  apply (smt assn_ext entailsD' entailsI mod_false' mult.left_neutral pure_assn_eq_conv)   
+  using entails_pure' entails_triv by blast 
 
 lemma extr: "pHeap h as n \<Turnstile> \<up>B = (pHeap h as n \<Turnstile> emp \<and> B)"
   using one_assn_rule pure_assn_rule by auto  
@@ -153,17 +307,22 @@ lemma R: "((s,s') \<in> Rs \<Longrightarrow> hn_refine (emp) (c s) (G s' s) R (a
   unfolding hn_refine_def by (auto simp: hn_ctxt_def pure_def extr)
 
 
+thm hnr_uRETURN_pass
+
+lemma moneq: "(\<lambda>s. RETURNT (0 < s)) = (\<lambda>s. RETURNT 0 \<bind> (%c. RETURNT (c < s)))"
+  by (auto intro!: pw_eqI)
 
 schematic_goal
   assumes "a = (whileT (\<lambda>s. s>0) (\<lambda>s. RETURNT (s-1)) (S::nat))"
   shows "hn_refine emp ?c ?\<Gamma> (pure Id) a"
-  unfolding assms
-  apply(subst WHILEIT_def[symmetric, where I=I])
-  apply(subst WHILEIT_to_monadic)
+  unfolding assms 
+  apply(subst WHILEIT_to_monadic) apply(subst moneq)
   apply(rule hn_monadic_WHILE_aux[where \<Gamma>="emp"])
-      apply (simp add: hn_ctxt_def pure_def k) 
+      apply (simp add: hn_ctxt_def pure_def k entailst_def ) 
   
-     apply simp
+     apply (simp del: nres_bind_left_identity)
+     apply(rule hnr_bind) 
+
      apply(rule hn_refine_cons_pre)
       prefer 2     
      apply(rule hnr_uRETURN_pass)
